doc/coq/Sound.v
@@ -1,7 +1,18 @@
 From MODULAR Require Export Abstract.
 From MODULAR Require Export Concrete.
 
-Fixpoint dy_ctx_bound C t :=
+Module Abs := Abstract.
+Module Conc := Concrete.
+
+Generalizable Variables CT.
+Generalizable Variables AT.
+
+Definition lt `{Conc.Time CT} (t1 : CT) (t2 : CT) :=
+  leb t1 t2 = true /\ eqb t1 t2 = false.
+
+Notation "t1 '<' t2" := (lt t1 t2).
+
+Fixpoint dy_ctx_bound `{Conc.Time CT} C t :=
   match C with
   | [||] => True
   | dy_c_lam _ t' C'
@@ -9,19 +20,13 @@ Fixpoint dy_ctx_bound C t :=
   | dy_c_letm _ CM C' => dy_ctx_bound CM t /\ dy_ctx_bound C' t
   end.
 
-Fixpoint p_bound p t :=
-  match p with
-  | [] => True
-  | hd :: tl => hd < t /\ p_bound tl t
-  end.
-
-Definition time_bound C st :=
+Definition time_bound `{Conc.Time CT} C st :=
   match st with
   | ST mem t =>
     dy_ctx_bound C t /\
-    (forall p (NBOUND : ~(p_bound p t)),
+    (forall p (NBOUND : ~(p < t)),
       mem p = None) /\
-    (forall p (BOUND : p_bound p t),
+    (forall p (BOUND : p < t),
       match mem p with
       | Some (Closure _ _ C') => dy_ctx_bound C' t
       | _ => True
@@ -29,78 +34,75 @@ Definition time_bound C st :=
   end.
 
 Lemma p_bound_or_not :
-  forall p t,
-    p_bound p t \/ ~(p_bound p t).
+  forall `{Conc.Time CT} (p : CT) t,
+    (p < t) \/ ~(p < t).
 Proof.
-  induction p.
-  - intros; left; simpl; eauto.
-  - intros; simpl.
-    specialize (IHp t). assert (H : a < t \/ ~ a < t). nia.
-    destruct IHp as [BOUND | NBOUND]; destruct H as [BOUND' | NBOUND'].
-    + left; split; eauto.
-    + right. unfold not. intros H; destruct H.
-      apply NBOUND' in H. contradiction H.
-    + right. unfold not. intros H; destruct H.
-      apply NBOUND in H0. contradiction H0.
-    + right. unfold not. intros H; destruct H.
-      apply NBOUND' in H. contradiction H.
+  intros. unfold "<". unfold not.
+  remember (leb p t) as le. remember (eqb p t) as eq.
+  destruct le; destruct eq.
+  - right. intros contra. destruct contra as [? contra]. inversion contra.
+  - left; eauto.
+  - symmetry in Heqeq. rewrite eqb_eq in Heqeq. subst.
+    rewrite leb_refl in Heqle. inversion Heqle.
+  - right. intros contra. destruct contra as [contra ?]. inversion contra.
 Qed.
 
-Definition trans_t := Concrete.time -> Abstract.time.
+Definition eq_bound_α 
+  `{Conc.Time CT} `{Abs.Time AT} t (α : CT -> AT) α' :=
+  forall t' (LE : leb t' t = true), α t' = α' t'.
 
-Definition eq_bound_α t (α : trans_t) α' :=
-  forall t' (LE : t' <= t), α t' = α' t'.
-
-Fixpoint trans_ctx (α : trans_t) C :=
+Fixpoint trans_ctx `{Conc.Time CT} `{Abs.Time AT} (α : CT -> AT) C :=
   match C with
-  | [||] => [#||#]
-  | dy_c_lam x t C' => Abstract.dy_c_lam x (α t) (trans_ctx α C')
-  | dy_c_lete x t C' => Abstract.dy_c_lete x (α t) (trans_ctx α C')
-  | dy_c_letm M CM C' => Abstract.dy_c_letm M (trans_ctx α CM) (trans_ctx α C')
+  | [||] => [||]
+  | dy_c_lam x t C' => dy_c_lam x (α t) (trans_ctx α C')
+  | dy_c_lete x t C' => dy_c_lete x (α t) (trans_ctx α C')
+  | dy_c_letm M CM C' => dy_c_letm M (trans_ctx α CM) (trans_ctx α C')
   end.
 
-Definition sound α C st abs_C abs_st :=
+Definition sound `{Conc.Time CT} `{Abs.Time AT} α C st abs_C abs_st :=
   match abs_st with
-  | Abstract.ST abs_mem abs_t =>
+  | Abs.ST abs_mem abs_t =>
     match st with
     | ST mem t =>
       α t = abs_t /\
       trans_ctx α C = abs_C /\
-      forall p (BOUND : p_bound p t),
+      forall p (BOUND : p < t),
         match mem p with
         | None => True
         | Some (Closure x e Cv) =>
-          let l := abs_mem (map α p) in
-          In (Abstract.Closure x e (trans_ctx α Cv)) l
+          let l := abs_mem (α p) in
+          In (Closure x e (trans_ctx α Cv)) l
         end
     end
   end.
 
 Lemma trans_ctx_addr :
-  forall α C x,
-    Abstract.addr_x (trans_ctx α C) x = List.map α (addr_x C x).
+  forall `{Conc.Time CT} `{Abs.Time AT} α C x,
+    addr_x (trans_ctx α C) x = 
+      match (addr_x C x) with 
+      | None => None 
+      | Some addr => Some (α addr) 
+      end.
 Proof.
   induction C; eauto.
   - intros. specialize (IHC x0).
     simpl. rewrite IHC.
     destruct (addr_x C x0); simpl; eauto.
     destruct (eq_eid x0 x); eauto.
-    rewrite map_app. eauto.
   - intros. specialize (IHC x0).
     simpl. rewrite IHC.
     destruct (addr_x C x0); simpl; eauto.
     destruct (eq_eid x0 x); eauto.
-    rewrite map_app. eauto.
 Qed.
 
 Lemma trans_ctx_ctx_M :
-  forall C α abs_C M C_M
+  forall `{Conc.Time CT} `{Abs.Time AT} C α abs_C M C_M
         (ACCESS : ctx_M C M = Some C_M)
         (TRANS : trans_ctx α C = abs_C),
-    Abstract.ctx_M abs_C M = Some (trans_ctx α C_M).
+    ctx_M abs_C M = Some (trans_ctx α C_M).
 Proof.
-  assert (forall C α M,
-    match Abstract.ctx_M (trans_ctx α C) M with
+  assert (forall `{Conc.Time CT} `{Abs.Time AT} C α M,
+    match ctx_M (trans_ctx α C) M with
     | Some _ => 
       match ctx_M C M with
       | Some _ => True
@@ -115,7 +117,7 @@ Proof.
   {
     induction C; intros; simpl; eauto; try apply IHC.
     destruct (eq_mid M0 M); 
-    remember (Abstract.ctx_M (trans_ctx α C2) M0) as ctx';
+    remember (ctx_M (trans_ctx α C2) M0) as ctx';
     destruct ctx';
     specialize (IHC2 α M0);
     rewrite <- Heqctx' in IHC2;
@@ -127,14 +129,14 @@ Proof.
   - rewrite <- TRANS. simpl. apply IHC; eauto.
   - rewrite <- TRANS. simpl. apply IHC; eauto. 
   - rewrite <- TRANS. simpl.
-    remember (Abstract.ctx_M (trans_ctx α C2) M0) as ctx1.
+    remember (ctx_M (trans_ctx α C2) M0) as ctx1.
     destruct ctx1; try (inversion ACCESS; fail).
-    + specialize (H C2 α M0).
+    + specialize (H CT H0 H1 AT H2 H3 C2 α M0).
       rewrite <- Heqctx1 in H.
       remember (ctx_M C2 M0) as ctx2; destruct ctx2;
       inversion H; inversion ACCESS; subst.
       rewrite Heqctx1. apply IHC2; eauto.
-    + specialize (H C2 α M0).
+    + specialize (H CT H0 H1 AT H2 H3 C2 α M0).
       rewrite <- Heqctx1 in H.
       remember (ctx_M C2 M0) as ctx2; destruct ctx2;
       inversion H; destruct (eq_mid M0 M);
@@ -142,12 +144,12 @@ Proof.
 Qed.
 
 Lemma time_increase_e :
-  forall C st e e' st'
+  forall `{Conc.Time CT} `{Abs.Time AT} C st e e' st'
          (EVAL : EvalR C st e e' st'),
     match st with
     | ST _ t =>
       match st' with
-      | ST _ t' => t <= t'
+      | ST _ t' => leb t t' = true
       end
     end.
 Proof.
@@ -155,90 +157,105 @@ Proof.
   induction EVAL;
   intros; 
   destruct st; try destruct st'; try destruct st''; try destruct st_v; 
-  try destruct st_m; try destruct st_lam;
-  unfold update_t in *; simpl; try nia.
+  try destruct st_m; try destruct st_lam; simpl; try apply leb_refl.
+  - inversion STATE; subst. apply leb_refl.
+  - assert (t < update C (ST mem t) x arg).
+    { apply update_lt. }
+    destruct H3. 
+    apply leb_trans with (t' := (update C (ST mem t) x arg)); eauto.
+    apply leb_trans with (t' := t); eauto.
+    apply leb_trans with (t' := t2); eauto.
+  - apply leb_trans with (t' := t1); eauto.
+  - assert (t < update C (ST mem t) x v).
+    { apply update_lt. }
+    destruct H3.
+    apply leb_trans with (t' := (update C (ST mem t) x v)); eauto.
+    apply leb_trans with (t' := t); eauto.
+  - apply leb_trans with (t' := t0); eauto.
 Qed.
 
 Lemma relax_ctx_bound :
-  forall C t1 t2 (BOUND : dy_ctx_bound C t1) (LE : t1 <= t2),
+  forall `{Conc.Time CT} `{Abs.Time AT} 
+         C t1 t2 (BOUND : dy_ctx_bound C t1) (LE : leb t1 t2 = true),
          dy_ctx_bound C t2.
 Proof.
   induction C; intros; destruct BOUND; simpl in *; 
-  repeat split; try nia;
-  try eapply IHC; try eapply IHC1; try eapply IHC2; eauto.
+  repeat split;
+  try eapply IHC; try eapply IHC1; try eapply IHC2; eauto;
+  try destruct H3; try apply leb_trans with (t' := t1); eauto.
+  rewrite eqb_neq in *. red. intros; subst. apply H5. apply leb_sym; eauto.
+  rewrite eqb_neq in *. red. intros; subst. apply H5. apply leb_sym; eauto.
 Qed.
 
 Lemma relax_p_bound :
-  forall p t1 t2 (BOUND : p_bound p t1) (LE : t1 <= t2),
-         p_bound p t2.
+  forall `{Conc.Time CT} `{Abs.Time AT}
+    p t1 t2 (BOUND : p < t1) (LE : leb t1 t2 = true),
+  p < t2.
 Proof.
-  induction p; intros; destruct BOUND; simpl in *; 
-  repeat split; try nia; eauto.
-Qed.
-
-Lemma p_bound_app :
-  forall p1 p2 t,
-    p_bound (p1 ++ p2) t <-> p_bound p1 t /\ p_bound p2 t.
-Proof.
-  induction p1; intros; split; intro H; try destruct H; simpl in *; eauto.
-  - rewrite IHp1 in H0. destruct H0. repeat split; eauto.
-  - rewrite IHp1. destruct H. repeat split; eauto.
+  intros. destruct BOUND. split.
+  apply leb_trans with (t' := t1); eauto.
+  rewrite eqb_neq. red. intros; subst.
+  assert (t1 = t2). apply leb_sym; eauto. subst.
+  assert (true = eqb t2 t2). symmetry. apply eqb_eq; eauto.
+  rewrite <- H5 in H4. inversion H4.
 Qed.
 
 Lemma time_bound_addr :
-  forall C x t,
-    dy_ctx_bound C t -> p_bound (addr_x C x) t.
+  forall `{Conc.Time CT} `{Abs.Time AT} C x t,
+    dy_ctx_bound C t -> 
+    match addr_x C x with
+    | None => True
+    | Some addr => addr < t
+    end.
 Proof.
-  induction C; intros; simpl in *; destruct H; eauto.
-  - specialize (IHC x0 t H0).
-    destruct (addr_x C x0). destruct (eq_eid x0 x); simpl; eauto.
-    rewrite p_bound_app with (p1 := t0 :: l) (p2 := [tx]).
-    split; simpl; eauto.
-  - specialize (IHC x0 t H0).
-    destruct (addr_x C x0). destruct (eq_eid x0 x); simpl; eauto.
-    rewrite p_bound_app with (p1 := t0 :: l) (p2 := [tx]).
-    split; simpl; eauto.
-Qed.
-
-Lemma time_bound_level :
-  forall C t,
-    dy_ctx_bound C t -> p_bound (dy_level C) t.
-Proof.
-  induction C; intros; simpl in *; destruct H;
-  try rewrite p_bound_app; try split; simpl; eauto.
+  induction C; intros; simpl in *; try destruct H3; eauto.
+  - specialize (IHC x0 t H4).
+    destruct (addr_x C x0); eauto. 
+    destruct (eq_eid x0 x); simpl; eauto.
+  - specialize (IHC x0 t H4).
+    destruct (addr_x C x0); eauto. 
+    destruct (eq_eid x0 x); simpl; eauto.
+  - apply IHC2; eauto.
 Qed.
 
 Lemma time_bound_ctx_M :
-  forall C M t CM,
+  forall `{Conc.Time CT} `{Abs.Time AT} C M t CM,
     ctx_M C M = Some CM ->
     dy_ctx_bound C t -> 
     dy_ctx_bound CM t.
 Proof.
   induction C; intros; simpl in *.
-  - inversion H.
-  - eapply IHC. exact H. destruct H0; eauto.
-  - eapply IHC. exact H. destruct H0; eauto.
+  - inversion H3.
+  - eapply IHC; eauto. destruct H4; eauto.
+  - eapply IHC; eauto. destruct H4; eauto.
   - remember (ctx_M C2 M0) as oCM.
     destruct oCM.
-    + eapply IHC2. symmetry. inversion H; subst. exact HeqoCM.
-      destruct H0; eauto.
-    + destruct (eq_mid M0 M); inversion H; subst.
-      destruct H0; eauto.
+    + inversion H3; subst. eapply IHC2; eauto.
+      destruct H4; eauto.
+    + destruct (eq_mid M0 M); inversion H3; subst.
+      destruct H4; eauto.
 Qed.
 
 Lemma plugin_ctx_bound :
-  forall Cout Cin t,
+  forall `{Conc.Time CT} `{Abs.Time AT} Cout Cin t,
     dy_ctx_bound (Cout[|Cin|]) t <-> dy_ctx_bound Cout t /\ dy_ctx_bound Cin t.
 Proof.
-  intros; split; intros H; induction Cout; repeat split; simpl in *; try nia; eauto;
-  destruct H as [H' H'']; try specialize (IHCout H'') as HINT;
-  try specialize (IHCout1 H'') as HINT; try specialize (IHCout2 H'') as HINT;
-  try destruct HINT; eauto;
-  try apply IHCout; destruct H'; try split; eauto.
+  intros. 
+  rename H into O1. rename H0 into T1. rename H1 into O2. rename H2 into T2.
+  revert Cout Cin t. induction Cout; repeat split; intros; simpl in *; 
+  try destruct H as [[LE NEQ] BD]; 
+  try destruct H as [BD1 BD2];
+  try (try apply IHCout with (Cin := Cin);
+       try apply IHCout1 with (Cin := Cin1);
+       try apply IHCout2 with (Cin := Cin2); eauto; fail);
+  try (destruct LE; eauto).
+  rewrite IHCout2 in BD2. destruct BD2; eauto.
+  rewrite IHCout2 in BD2. destruct BD2; eauto.
+  rewrite IHCout2; eauto.
 Qed.
 
 Lemma time_bound_e :
-  forall C st e e' st'
+  forall `{Conc.Time CT} `{Abs.Time AT} C st e e' st'
          (EVAL : EvalR C st e e' st')
          (BOUND : time_bound C st),
     match e' with
@@ -246,12 +263,16 @@ Lemma time_bound_e :
     | MVal C' => time_bound C' st'
     end.
 Proof.
-  intros. induction EVAL; intros; simpl; eauto.
+  intros. 
+  rename H into O1. rename H0 into T1.
+  rename H1 into O2. rename H2 into T2.
+  induction EVAL; intros; simpl; eauto.
   - destruct v. unfold time_bound in *.
     destruct st. destruct BOUND as [? [? RR]].
-    specialize (RR (addr_x C x)) as RR'.
-    assert (p_bound (addr_x C x) t0). apply time_bound_addr. eauto.
-    apply RR' in H1. inversion STATE; subst. 
+    specialize (RR addr) as RR'. inversion STATE; subst.
+    pose proof (time_bound_addr C x t0 H).
+    rewrite <- ADDR in H1.
+    apply RR' in H1. 
     rewrite <- ACCESS in H1. repeat split; eauto.
   - specialize (IHEVAL1 BOUND). 
     destruct v. destruct arg. 
@@ -267,37 +288,36 @@ Proof.
       simpl in BOUND. destruct BOUND. exact d. eauto. 
     }
     specialize (IHEVAL2 HINT).
-    assert (p_bound (t :: dy_level C_lam) (update_t C (ST mem t) x (Closure x1 e3 C1))).
-    {
-      simpl in IHEVAL1. destruct IHEVAL1 as [? [? ?]].
-      simpl. split; unfold update_t; eauto.
-      apply relax_p_bound with (t1 := t1).
-      apply time_bound_level. eauto. nia.
-    }
+    assert (t < (update C (ST mem t) x (Closure x1 e3 C1))).
+    { apply update_lt. }
     apply IHEVAL3; simpl. split.
     rewrite plugin_ctx_bound. split.
     simpl in IHEVAL1. destruct IHEVAL1 as [? [? ?]].
-    eapply relax_ctx_bound. eauto. nia.
+    eapply relax_ctx_bound. eauto. destruct H.
+    apply leb_trans with (t' := t); eauto.
     simpl. split; eauto.
     split; intros;
-    unfold update_m; remember (eq_p p (t :: dy_level C_lam)) as b;
-    destruct b; symmetry in Heqb; try rewrite eq_p_eq in Heqb.
-    + assert (p_bound p (S t)) as contra. { rewrite Heqb. eauto. }
+    unfold update_m; remember (eqb p t) as b;
+    destruct b; symmetry in Heqb; try rewrite eqb_eq in Heqb.
+    + assert (p < update C (ST mem t) x (Closure x1 e3 C1)) as contra. 
+      { rewrite Heqb. destruct H; split; eauto. }
       apply NBOUND in contra. inversion contra.
     + simpl in IHEVAL2. destruct IHEVAL2 as [? [RR ?]].
-      apply RR. unfold not. intros. 
-      assert (p_bound p (S t)) as contra.
-      apply relax_p_bound with (t1 := t); eauto. 
+      apply RR. unfold not. intros.
+      assert (p < update C (ST mem t) x (Closure x1 e3 C1)) as contra.
+      apply relax_p_bound with (t1 := t); try assumption.
+      apply update_lt.
       apply NBOUND in contra. inversion contra.
-    + apply relax_ctx_bound with (t1 := t); eauto.
+    + apply relax_ctx_bound with (t1 := t).
       simpl in IHEVAL2. destruct IHEVAL2 as [? [? ?]]; eauto.
+      apply update_lt.
     + destruct IHEVAL2 as [? [? RR]]. 
       specialize (RR p). remember (mem p) as access eqn:ACCESS.
       destruct access; eauto. destruct e4.
-      apply relax_ctx_bound with (t1 := t); eauto. apply RR.
+      apply relax_ctx_bound with (t1 := t). apply RR. split; try assumption.
       pose proof (p_bound_or_not p t) as CASES.
-      destruct CASES as [? | contra]; eauto.
-      specialize (H1 p contra). rewrite H1 in ACCESS. inversion ACCESS.
+      destruct CASES as [? | contra]. apply H2.
+      specialize (H1 p contra). rewrite H1 in ACCESS. inversion ACCESS. apply H.
   - apply IHEVAL2. apply IHEVAL1. eauto.
   - destruct st. simpl in *. destruct BOUND as [? [? ?]].
     repeat split; eauto. eapply time_bound_ctx_M.
@@ -307,34 +327,27 @@ Proof.
     destruct st. destruct st_m.
     apply time_increase_e in EVAL1 as time_inc1.
     apply time_increase_e in EVAL2 as time_inc2.
-    assert (p_bound (t :: dy_level C) (update_t C (ST mem t) x (Closure x0 e0 C0))).
-    {
-      simpl in BOUND. destruct BOUND as [? [? ?]].
-      simpl. split; unfold update_t; eauto.
-      apply relax_p_bound with (t1 := t0).
-      apply time_bound_level. eauto. nia.
-    }
     simpl in BOUND. destruct BOUND as [B1 [B2 B3]].
     simpl in IHEVAL1. destruct IHEVAL1 as [HH1 [HH2 HH3]].
     apply IHEVAL2. simpl; split.
     rewrite plugin_ctx_bound; split.
-    apply relax_ctx_bound with (t1 := t0); eauto. simpl; split; eauto.
+    apply relax_ctx_bound with (t1 := t0); eauto. 
+    apply leb_trans with (t' := t); try assumption. apply update_lt. 
+    simpl; split; eauto. apply update_lt.
     split; intros;
-    unfold update_m; remember (eq_p p (t :: dy_level C)) as b;
-    destruct b; symmetry in Heqb; try rewrite eq_p_eq in Heqb.
-    + assert (p_bound p (S t)) as contra. { rewrite Heqb. eauto. }
-      apply NBOUND in contra. inversion contra.
+    unfold update_m; remember (eqb p t) as b;
+    destruct b; symmetry in Heqb; try rewrite eqb_eq in Heqb.
+    + subst. assert False as contra. apply NBOUND. apply update_lt. inversion contra.
     + apply HH2. unfold not. intros. 
-      assert (p_bound p (S t)) as contra.
-      apply relax_p_bound with (t1 := t); eauto. 
-      apply NBOUND in contra. inversion contra.
-    + apply relax_ctx_bound with (t1 := t); eauto.
+      assert False as contra. apply NBOUND.
+      apply relax_p_bound with (t1 := t); try assumption. apply update_lt. eauto.
+    + subst. apply relax_ctx_bound with (t1 := t); try assumption. apply update_lt.
     + specialize (HH3 p). remember (mem p) as access eqn:ACCESS.
       destruct access; eauto. destruct e1.
-      apply relax_ctx_bound with (t1 := t); eauto. apply HH3.
+      apply relax_ctx_bound with (t1 := t); try assumption. apply HH3.
       pose proof (p_bound_or_not p t) as CASES.
       destruct CASES as [? | contra]; eauto.
-      specialize (HH2 p contra). rewrite HH2 in ACCESS. inversion ACCESS.
+      specialize (HH2 p contra). rewrite HH2 in ACCESS. inversion ACCESS. apply update_lt.
   - specialize (IHEVAL1 BOUND).
     destruct st. destruct st'. destruct st''.
     simpl in BOUND. destruct BOUND as [B1 [B2 B3]].
@@ -348,8 +361,8 @@ Proof.
 Qed.
 
 Lemma plugin_trans_ctx :
-  forall Cout Cin α,
-    trans_ctx α (Cout[|Cin|]) = (trans_ctx α Cout [#|trans_ctx α Cin|#]).
+  forall `{Conc.Time CT} `{Abs.Time AT} Cout Cin α,
+    trans_ctx α (Cout[|Cin|]) = (trans_ctx α Cout [|trans_ctx α Cin|]).
 Proof.
   induction Cout; intros; simpl; 
   try rewrite IHCout; try rewrite IHCout1; try rewrite IHCout2;
@@ -357,35 +370,58 @@ Proof.
 Qed.
 
 Lemma bound_trans_ctx_eq :
-  forall C t α α',
+  forall `{Conc.Time CT} `{Abs.Time AT} C t α α',
          dy_ctx_bound C t ->
          eq_bound_α t α α' ->
          trans_ctx α C = trans_ctx α' C.
 Proof.
-  intros.
+  intros. 
+  rename H into O1. rename H0 into T1.
+  rename H1 into O2. rename H2 into T2.
   induction C; simpl; try rewrite IHC; 
   try rewrite IHC1; try rewrite IHC2; simpl in *; eauto;
-  destruct H; eauto.
-  unfold eq_bound_α in H0. rewrite H0; eauto. nia.
-  unfold eq_bound_α in H0. rewrite H0; eauto. nia.
+  destruct H3; eauto; inversion H.
+  unfold eq_bound_α in H0. rewrite H4; eauto.
+  unfold eq_bound_α in H0. rewrite H4; eauto.
 Qed.
 
-Lemma level_trans_ctx_eq :
-  forall C α α' t,
-    eq_bound_α t α α' ->
-    dy_ctx_bound C t ->
-    Abstract.dy_level (trans_ctx α C) = map α' (dy_level C).
+Ltac contradict :=
+  let contra := fresh "contra" in
+  assert False as contra; eauto 3; inversion contra.
+
+Lemma __R__ : forall b, b = false <-> ~ b = true.
+Proof. 
+  intros; destruct b; unfold "<>"; split; 
+  intros; try inversion H; try inversion H0; try contradict; eauto.
+Qed.
+
+Ltac refl_bool :=
+  match goal with
+  | |- _ = false => rewrite __R__
+  | |- _ <> true => rewrite <- __R__
+  | _ => idtac
+  end.
+
+Ltac lebt x :=
+  apply leb_trans with (t' := x); try assumption; try apply update_lt.
+
+Lemma eqb_refl : forall `{OrderT CT} t, eqb t t = true.
 Proof.
-  induction C; intros; simpl; eauto; try rewrite map_app; simpl;
-  try erewrite IHC; simpl in H0; destruct H0; eauto.
-  - assert (α tx = α' tx). red in H. apply H. nia. rewrite H0. eauto.
-  - assert (α tx = α' tx). red in H. apply H. nia. rewrite H0. eauto.
+  intros. rewrite eqb_eq. eauto.
+Qed.
+
+Lemma eqb_update : forall `{Conc.Time CT} C mem t x x' e' C',
+  eqb t (update C (ST mem t) x (Closure x' e' C')) = false.
+Proof.
+  intros. refl_bool. unfold "<>". intros.
+  assert (t < update C (ST mem t) x (Closure x' e' C')) as contra. apply update_lt.
+  destruct contra as [? contra]. rewrite contra in *. inversion H1.
 Qed.
 
 (* Set Printing Implicit. *)
 
 Lemma sound_eval :
-  forall C st e v' st'
+  forall `{Conc.Time CT} `{Abs.Time AT} C st e v' st'
          (EVAL : EvalR C st e v' st')
          (BOUND : time_bound C st)
          abs_C abs_st α
@@ -397,40 +433,40 @@ Lemma sound_eval :
         match v' with
         | EVal (Closure x' e' C') =>
           sound α' C' st' abs_C' abs_st' /\
-          Abstract.EvalR 
+          Abs.EvalR 
             abs_C abs_st e 
-            (Abstract.EVal (Abstract.Closure x' e' (trans_ctx α' C')))
+            (EVal (Closure x' e' (trans_ctx α' C')))
             abs_st'
         | MVal C' =>
           sound α' C' st' abs_C' abs_st' /\
-          Abstract.EvalR 
+          Abs.EvalR 
             abs_C abs_st e 
-            (Abstract.MVal (trans_ctx α' C'))
+            (MVal (trans_ctx α' C'))
             abs_st' 
         end
       end.
 Proof.
-  intros. revert abs_C abs_st α SOUND. induction EVAL; intros; subst.
+  intros. rename H into O1. rename H0 into T1. rename H1 into O2. rename H2 into T2.
+  revert abs_C abs_st α SOUND. induction EVAL; intros; subst.
   - unfold sound in SOUND. destruct abs_st as [abs_mem abs_t].
     destruct SOUND as [? [? ?]].
-    specialize (H1 (addr_x C x)) as HINT. rewrite <- ACCESS in HINT.
-    destruct v as [v pf C'].
-    exists (trans_ctx α C'). exists (Abstract.ST abs_mem abs_t). exists α.
+    specialize (H1 addr) as HINT. rewrite <- ACCESS in HINT.
+    destruct v as [v e C'].
+    exists (trans_ctx α C'). exists (Abs.ST abs_mem abs_t). exists α.
     repeat split; try red; intros; eauto. apply H1. eauto.
-    eapply Abstract.Eval_var_e; eauto.
+    apply Abs.Eval_var_e with (addr := α addr) (mem := abs_mem) (t := abs_t); eauto.
     rewrite <- H0. rewrite trans_ctx_addr.
-    destruct (addr_x C x). specialize (ADDR eq_refl). inversion ADDR.
-    simpl; unfold not; intros contra; inversion contra.
-    rewrite <- H0. rewrite trans_ctx_addr.
-    apply HINT. simpl in BOUND. destruct BOUND. apply time_bound_addr. eauto.
-  - exists abs_C. exists abs_st. exists α. repeat split; eauto using Abstract.EvalR.
+    destruct (addr_x C x); inversion ADDR; subst; eauto.
+    apply HINT. simpl in BOUND. destruct BOUND.
+    pose proof (time_bound_addr C x t H2). rewrite <- ADDR in *. eauto.
+  - exists abs_C. exists abs_st. exists α. repeat split; eauto.
     destruct st; simpl; repeat split; try red; intros; eauto.
     destruct abs_st. simpl in SOUND. destruct SOUND as [? [? ?]].
-    rewrite H0. eauto using Abstract.EvalR.
+    rewrite H0. eauto.
   - pose proof (time_bound_e C st e1 (EVal (Closure x e C_lam)) st_lam EVAL1) as BOUND'.
     pose proof (time_bound_e C st_lam e2 (EVal arg) (ST mem t) EVAL2) as BOUND''.
     pose proof (time_bound_e (C_lam [|dy_c_lam x t ([||])|])
-                             (ST (t :: dy_level C_lam !-> arg; mem) (update_t C (ST mem t) x arg))
+                             (ST (t !-> arg; mem) (update C (ST mem t) x arg))
                              e (EVal v) st_v EVAL3) as BOUND'''.
     specialize (BOUND' BOUND). simpl in BOUND'.
     destruct st. destruct st_lam. destruct st_v.
@@ -445,27 +481,27 @@ Proof.
     specialize (BOUND'' B1).
     destruct arg. destruct v.
     assert (time_bound (C_lam [|dy_c_lam x t ([||])|])
-             (ST (t :: dy_level C_lam !-> Closure x0 e0 C0; mem)
-                (update_t C (ST mem t) x (Closure x0 e0 C0)))) as B2.
+             (ST (t !-> Closure x0 e0 C0; mem)
+                (update C (ST mem t) x (Closure x0 e0 C0)))) as B2.
     { simpl. simpl in BOUND. destruct BOUND as [BB1 [BB2 BB3]].
              simpl in BOUND'. destruct BOUND' as [BB1' [BB2' BB3']].
              simpl in BOUND''. destruct BOUND'' as [BB1'' [BB2'' BB3'']].
-      unfold update_t in *.
       split. rewrite plugin_ctx_bound. split.
-      eapply relax_ctx_bound. eauto. eauto. simpl. split; eauto. split.
+      eapply relax_ctx_bound. eauto. lebt t.
+      simpl. split; eauto. split. apply update_lt. apply update_lt. split.
       (* not bound, then None *)
-      intros. unfold update_m. remember (eq_p p (t :: dy_level C_lam)) as b.
-      destruct b. symmetry in Heqb. rewrite eq_p_eq in Heqb.
+      intros. unfold update_m. remember (eqb p t) as b.
+      destruct b. symmetry in Heqb. rewrite eqb_eq in Heqb.
       rewrite Heqb in NBOUND. simpl in NBOUND.
-      assert (t < S t /\ p_bound (dy_level C_lam) (S t)) as contra.
-      split; eauto. apply time_bound_level. apply relax_ctx_bound with (t1 := t1). eauto. eauto.
-      apply NBOUND in contra. inversion contra.
-      apply BB2''. unfold not. intros contra.
-      assert (p_bound p (S t)). apply relax_p_bound with (t1 := t); eauto.
-      apply NBOUND in H. inversion H.
+      assert False as contra. apply NBOUND. apply update_lt. inversion contra.
+      apply BB2''. unfold not. intros [LE NEQ].
+      apply NBOUND. split. lebt t.
+      refl_bool. unfold "<>". intros contra. rewrite eqb_eq in *.
+      assert (t = p) as RR. apply leb_sym; try assumption. rewrite contra. apply update_lt.
+      rewrite eqb_neq in NEQ. apply NEQ; eauto.
       (* bound, then access is bound *)
-      intros. unfold update_m. remember (eq_p p (t :: dy_level C_lam)) as b.
-      destruct b. symmetry in Heqb. rewrite eq_p_eq in Heqb.
+      intros. unfold update_m. remember (eqb p t) as b.
+      destruct b. symmetry in Heqb. rewrite eqb_eq in Heqb.
       rewrite Heqb in BOUND. simpl in BOUND. destruct BOUND.
       apply relax_ctx_bound with (t1 := t); eauto.
       pose proof (p_bound_or_not p t) as CASES.
@@ -473,7 +509,7 @@ Proof.
       destruct CASES; destruct access; try destruct e4; eauto;
       try specialize (BB2'' p H); try specialize (BB3'' p H);
       try rewrite <- ACCESS in BB2''; try rewrite <- ACCESS in BB3'';
-      try apply relax_ctx_bound with (t1 := t); eauto. inversion BB2''. }
+      try apply relax_ctx_bound with (t1 := t); try apply update_lt. eauto. inversion BB2''. }
     specialize (BOUND''' B2).
     specialize (IHEVAL1 BOUND). specialize (IHEVAL2 B1). specialize (IHEVAL3 B2). 
     specialize (IHEVAL1 abs_C abs_st α SOUND).
@@ -485,80 +521,72 @@ Proof.
       eauto. eauto. }
     specialize (IHEVAL2 abs_C abs_st' α' H). clear H.
     destruct IHEVAL2 as [abs_C'' [abs_st'' [α'' [EQ'' SOUND'']]]]. destruct abs_st'' as [mem'' t''].
-    remember (fun (t' : nat) => if t' =? S t 
-                        then Abstract.update_t abs_C (Abstract.ST mem'' t'') 
-                                                x (Abstract.Closure x0 e0 abs_C'') 
+    remember (fun t' => if eqb t' (update C (ST mem t) x (Closure x0 e0 C0))
+                        then Abs.update abs_C (Abs.ST mem'' t'') x (Closure x0 e0 abs_C'') 
                         else α'' t') as α'''.
+    assert (eq_bound_α t α'' α''') as EQ'''.
+    { red. intros. rewrite Heqα'''. 
+      assert (eqb t' (update C (ST mem t) x (Closure x0 e0 C0)) = false) as RR.
+      refl_bool. unfold "<>". intros contra. rewrite eqb_eq in contra.
+      assert (leb t t' = true). rewrite contra. apply update_lt. 
+      assert (t = t') as RR. apply leb_sym; eauto. rewrite <- RR in contra.
+      clear RR.
+      assert (eqb t (update C (ST mem t) x (Closure x0 e0 C0)) <> true).
+      refl_bool. apply update_lt. apply H0. rewrite <- contra. apply eqb_refl.
+      rewrite RR. eauto. }
     assert (sound α''' (C_lam [|dy_c_lam x t ([||])|])
-            (ST (t :: dy_level C_lam !-> Closure x0 e0 C0; mem) 
-                (update_t C (ST mem t) x (Closure x0 e0 C0)))
-            (abs_C'[#| Abstract.dy_c_lam x (α'' t) ([#||#]) |#])
-            (Abstract.ST ((α'' t) :: Abstract.dy_level abs_C' !#-> Abstract.Closure x0 e0 abs_C''; mem'') 
-                         (Abstract.update_t abs_C (Abstract.ST mem'' t'') x (Abstract.Closure x0 e0 abs_C'')))).
-    { simpl. unfold update_t in *. repeat split.
-      - rewrite Heqα'''. simpl. assert (t =? t = true). rewrite Nat.eqb_eq. eauto. rewrite H. eauto.
-      - rewrite Heqα'''. simpl. rewrite plugin_trans_ctx; simpl.
-        assert (t =? S t = false). rewrite Nat.eqb_neq. eauto. rewrite H.
+            (ST (t !-> Closure x0 e0 C0; mem) 
+                (update C (ST mem t) x (Closure x0 e0 C0)))
+            (abs_C'[| dy_c_lam x (α'' t) ([||]) |])
+            (Abs.ST ((α'' t) !#-> Closure x0 e0 abs_C''; mem'') 
+                    (Abs.update abs_C (Abs.ST mem'' t'') x (Closure x0 e0 abs_C'')))).
+    { simpl. repeat split.
+      - rewrite Heqα'''. rewrite eqb_refl. eauto.
+      - rewrite plugin_trans_ctx; simpl. rewrite Heqα'''.
+        rewrite eqb_update. rewrite <- Heqα'''.
         assert (trans_ctx α''' C_lam = abs_C'). rewrite Heqα'''.
-        destruct abs_st'. simpl in SOUND'. destruct SOUND' as [[? [? ?]] ?]. rewrite <- H1.
-        apply bound_trans_ctx_eq with (t := t1). simpl in BOUND'. destruct BOUND'. eauto.
-        red. intros. assert (t' <> S t). nia. rewrite <- Nat.eqb_neq in H4. rewrite H4.
-        symmetry. apply EQ''. eauto. 
-        rewrite Heqα''' in H0. simpl in H0. rewrite H0. eauto.
+        destruct abs_st'. simpl in SOUND'. destruct SOUND' as [[? [? ?]] ?]. rewrite <- H0.
+        apply bound_trans_ctx_eq with (t := t1). apply BOUND'.
+        red. intros. assert (eqb t' (update C (ST mem t) x (Closure x0 e0 C0)) = false).
+        refl_bool. unfold "<>". intros contra. rewrite eqb_eq in contra.
+        assert (leb t' t = true). lebt t1.
+        assert (t = t') as RR. apply leb_sym; try assumption. rewrite contra. apply update_lt.
+        assert (t < t') as contra'. rewrite contra. apply update_lt.
+        destruct contra' as [? contra']. rewrite RR in contra'. rewrite eqb_refl in contra'. inversion contra'.
+        rewrite H3. symmetry. apply EQ''. assumption. rewrite H. eauto.
       - intros. simpl in SOUND''. destruct SOUND'' as [[? [? ?]] ?].
         destruct abs_st'. simpl in SOUND'. destruct SOUND' as [[? [? ?]] ?].
-        unfold update_m. unfold Abstract.update_m.
-        remember (eq_p p (t :: dy_level C_lam)) as b.
-        destruct b. symmetry in Heqb. rewrite eq_p_eq in Heqb.
-        assert (map α''' p =  α'' t :: Abstract.dy_level abs_C').
-        rewrite Heqα'''. rewrite Heqb. simpl. assert (RR : t =? S t = false). 
-        apply Nat.eqb_neq. eauto. rewrite RR. clear RR. rewrite <- H4.
-        assert (Abstract.dy_level (trans_ctx α' C_lam) = map α''' (dy_level C_lam)) as RR.
-        apply level_trans_ctx_eq with (t := t1). red. intros.
-        assert (t' =? S t = false). rewrite Nat.eqb_neq. nia.
-        rewrite Heqα'''. rewrite H7. apply EQ''. eauto.
-        simpl in BOUND'. destruct BOUND'. eauto.
-        rewrite RR. rewrite Heqα'''. simpl. eauto.
-        (* A bug? in Coq : have to write explicitly the implicit parameters *)
-        assert (Abstract.eq_p (@map time Abstract.time α''' p) (@map nat bool α''' p) = true).
-        rewrite Abstract.eq_p_eq. eauto. rewrite <- H7. rewrite H8. simpl. left.
-        assert (abs_C'' = trans_ctx α''' C0).
-        rewrite <- H0. eapply bound_trans_ctx_eq. simpl in BOUND''. destruct BOUND''. eauto.
-        rewrite Heqα'''. red. intros. assert (t' =? S t = false). rewrite Nat.eqb_neq. nia.
-        rewrite H9. eauto. rewrite H9. eauto.
+        unfold update_m. unfold Abs.update_m.
+        remember (eqb p t) as b.
+        destruct b. symmetry in Heqb. rewrite eqb_eq in Heqb.
+        assert (eqb (α''' p) (α'' t) = true) as RR.
+        rewrite Heqα'''. rewrite Heqb. rewrite eqb_update. apply eqb_refl.
+        rewrite RR. clear RR. simpl. left. rewrite <- H0.
+        assert (trans_ctx α'' C0 = trans_ctx α''' C0) as RR.
+        apply bound_trans_ctx_eq with (t := t); eauto. apply BOUND''. rewrite RR; eauto.
         pose proof (p_bound_or_not p t) as CASES.
-        simpl in BOUND''. destruct BOUND'' as [B1'' [B2'' B3'']].
+        destruct BOUND'' as [B1'' [B2'' B3'']].
         destruct CASES as [L | R]; 
         try (specialize (B2'' p R); rewrite B2''; eauto; fail).
         remember (mem p) as access eqn: ACCESS.
         destruct access; eauto; destruct e4; simpl.
         specialize (H1 p L) as HINT. rewrite <- ACCESS in HINT.
-        assert (@map time Abstract.time α''' p = map α'' p) as RR. 
-        { clear HINT. clear BOUND0. clear Heqb. clear ACCESS.
-          induction p; simpl; eauto. simpl in L; destruct L.
-          rewrite IHp; eauto. rewrite Heqα'''. 
-          assert (a =? S t = false). rewrite Nat.eqb_neq. nia.
-          rewrite H9. eauto. } rewrite RR; clear RR.
-        assert (trans_ctx α''' C2 = trans_ctx α'' C2) as RR.
-        { apply bound_trans_ctx_eq with (t := t).
-          specialize (B3'' p L). rewrite <- ACCESS in B3''. eauto.
-          rewrite Heqα'''. red. intros. assert (t' =? S t = false).
-          rewrite Nat.eqb_neq. nia. rewrite H7. eauto. } rewrite RR; clear RR.
-        remember (α'' t :: Abstract.dy_level abs_C') as p'.
-        remember (Abstract.eq_p (map α'' p) p') as b.
+        assert (α''' p = α'' p) as RR. 
+        { symmetry. apply EQ'''. apply L. } rewrite RR; clear RR.
+        assert (trans_ctx α'' C2 = trans_ctx α''' C2) as RR.
+        { apply bound_trans_ctx_eq with (t := t); eauto.
+          specialize (B3'' p L). rewrite <- ACCESS in B3''. exact B3''. } rewrite <- RR; clear RR.
+        remember (α'' t) as p'.
+        remember (eqb (α'' p) p') as b.
         destruct b. 
-        simpl. right. symmetry in Heqb0. rewrite Abstract.eq_p_eq in Heqb0.
-        rewrite <- Heqb0. apply HINT. apply HINT.
+        simpl. right. symmetry in Heqb0. rewrite eqb_eq in Heqb0.
+        rewrite <- Heqb0. apply HINT; eauto. apply HINT; eauto.
     }
-    assert (eq_bound_α t α'' α''') as EQ'''.
-    { red. intros. rewrite Heqα'''. assert (t' =? S t = false). rewrite Nat.eqb_neq. nia.
-      rewrite H0. eauto. }
-    specialize (IHEVAL3 (abs_C' [#|Abstract.dy_c_lam x (α'' t) ([#||#])|#])
-                (Abstract.ST
-                  (α'' t :: Abstract.dy_level abs_C'
-                      !#-> Abstract.Closure x0 e0 abs_C''; mem'')
-                  (Abstract.update_t abs_C (Abstract.ST mem'' t'') x
-                  (Abstract.Closure x0 e0 abs_C''))) α''' H).
+    specialize (IHEVAL3 (abs_C' [|dy_c_lam x (α'' t) ([||])|])
+                (Abs.ST
+                  (α'' t !#-> Closure x0 e0 abs_C''; mem'')
+                  (Abs.update abs_C (Abs.ST mem'' t'') x
+                  (Closure x0 e0 abs_C''))) α''' H).
     destruct IHEVAL3 as [abs_C''' [abs_st''' [α'''' [EQ'''' SOUND''']]]].
     destruct SOUND' as [SOUND' EVAL'].
     destruct SOUND'' as [SOUND'' EVAL''].
@@ -566,9 +594,9 @@ Proof.
     exists abs_C'''. exists abs_st'''. exists α''''. repeat split; eauto.
     red. intros. 
     assert (α t' = α' t') as RR. apply EQ'. eauto. rewrite RR; clear RR.
-    assert (α' t' = α'' t') as RR. apply EQ''. nia. rewrite RR; clear RR.
-    assert (α'' t' = α''' t') as RR. apply EQ'''. nia. rewrite RR; clear RR.
-    apply EQ''''. unfold update_t. nia.
+    assert (α' t' = α'' t') as RR. apply EQ''. lebt t0. rewrite RR; clear RR.
+    assert (α'' t' = α''' t') as RR. apply EQ'''. lebt t1. lebt t0. rewrite RR; clear RR.
+    apply EQ''''. lebt t. lebt t1. lebt t0. 
     eapply Abstract.Eval_app. exact EVAL'. exact EVAL''.
     destruct abs_st'. simpl in SOUND'. destruct SOUND' as [? [RR ?]].
     rewrite RR. simpl in SOUND''. destruct SOUND'' as [? [RR' ?]].
@@ -588,7 +616,7 @@ Proof.
     destruct SOUND'' as [SOUND'' EVAL''].
     exists abs_C''. exists abs_st''. exists α''. repeat split; eauto.
     unfold eq_bound_α in *. intros.
-    assert (α'' t' = α' t'). symmetry. apply EQ''. nia.
+    assert (α'' t' = α' t'). symmetry. apply EQ''. lebt t.
     rewrite H. apply EQ'. eauto.
     eapply Abstract.Eval_link. eauto.
     destruct abs_st'. simpl in SOUND'. destruct SOUND' as [? [RR ?]].
@@ -596,41 +624,39 @@ Proof.
   - exists abs_C. exists abs_st. exists α. destruct st.
     repeat split; eauto. unfold eq_bound_α; intros; eauto.
     destruct abs_st. simpl in SOUND. destruct SOUND as [? [RR ?]].
-    rewrite RR. eauto using Abstract.EvalR.
+    rewrite RR. eauto.
   - exists (trans_ctx α C_M). exists abs_st. exists α. destruct st.
     destruct abs_st. destruct SOUND as [? [RR ?]].
     repeat split; eauto. rewrite <- RR.
     eapply Abstract.Eval_var_m. erewrite trans_ctx_ctx_M; eauto.
   - pose proof (time_bound_e C st e (EVal v) (ST mem t) EVAL1) as BOUND'.
     pose proof (time_bound_e (C [|dy_c_lete x t ([||])|]) 
-                             (ST (t :: dy_level C !-> v; mem)
-                                 (update_t C (ST mem t) x v)) m
+                             (ST (t !-> v; mem)
+                                 (update C (ST mem t) x v)) m
                              (MVal C_m) st_m EVAL2) as BOUND''.
     specialize (BOUND' BOUND). simpl in BOUND'.
     destruct st. destruct st_m. destruct v.
     apply time_increase_e in EVAL1 as time_inc1.
     apply time_increase_e in EVAL2 as time_inc2.
     assert (time_bound (C [|dy_c_lete x t ([||])|])
-            (ST (t :: dy_level C !-> (Closure x0 e0 C0); mem)
-               (update_t C (ST mem t) x (Closure x0 e0 C0)))) as B1.
+            (ST (t !-> (Closure x0 e0 C0); mem)
+               (update C (ST mem t) x (Closure x0 e0 C0)))) as B1.
     { simpl. simpl in BOUND. destruct BOUND as [BB1 [BB2 BB3]].
              simpl in BOUND'. destruct BOUND' as [BB1' [BB2' BB3']].
-      unfold update_t in *.
       split. rewrite plugin_ctx_bound. split.
-      eapply relax_ctx_bound. eauto. eauto. simpl. split; eauto. split.
+      eapply relax_ctx_bound. eauto. lebt t. simpl. split; eauto. apply update_lt. split.
       (* not bound, then None *)
-      intros. unfold update_m. remember (eq_p p (t :: dy_level C)) as b.
-      destruct b. symmetry in Heqb. rewrite eq_p_eq in Heqb.
-      rewrite Heqb in NBOUND. simpl in NBOUND.
-      assert (t < S t /\ p_bound (dy_level C) (S t)) as contra.
-      split; eauto. apply time_bound_level. apply relax_ctx_bound with (t1 := t0). eauto. eauto.
-      apply NBOUND in contra. inversion contra.
-      apply BB2'. unfold not. intros contra.
-      assert (p_bound p (S t)). apply relax_p_bound with (t1 := t); eauto.
-      apply NBOUND in H. inversion H.
+      intros. unfold update_m. remember (eqb p t) as b.
+      destruct b. symmetry in Heqb. rewrite eqb_eq in Heqb. 
+      assert False as contra. apply NBOUND. rewrite Heqb. apply update_lt. inversion contra.
+      apply BB2'. unfold not. intros [LE NEQ].
+      apply NBOUND. split. lebt t.
+      refl_bool. unfold "<>". intros contra. rewrite eqb_eq in *.
+      assert (t = p) as RR. apply leb_sym; try assumption. rewrite contra. apply update_lt.
+      rewrite eqb_neq in NEQ. apply NEQ; eauto.
       (* bound, then access is bound *)
-      intros. unfold update_m. remember (eq_p p (t :: dy_level C)) as b.
-      destruct b. symmetry in Heqb. rewrite eq_p_eq in Heqb.
+      intros. unfold update_m. remember (eqb p t) as b.
+      destruct b. symmetry in Heqb. rewrite eqb_eq in Heqb.
       rewrite Heqb in BOUND. simpl in BOUND. destruct BOUND.
       apply relax_ctx_bound with (t1 := t); eauto.
       pose proof (p_bound_or_not p t) as CASES.
@@ -638,53 +664,57 @@ Proof.
       destruct CASES; destruct access; try destruct e1; eauto;
       try specialize (BB2' p H); try specialize (BB3' p H);
       try rewrite <- ACCESS in BB2'; try rewrite <- ACCESS in BB3';
-      try apply relax_ctx_bound with (t1 := t); eauto. inversion BB2'. }
+      try apply relax_ctx_bound with (t1 := t); try apply update_lt; eauto. inversion BB2'. }
     specialize (BOUND'' B1).
     specialize (IHEVAL1 BOUND). specialize (IHEVAL2 B1).
     specialize (IHEVAL1 abs_C abs_st α SOUND).
     destruct IHEVAL1 as [abs_C' [abs_st' [α' [EQ' SOUND']]]].
-    remember (fun (t' : nat) => if t' =? S t 
-                        then Abstract.update_t abs_C abs_st'
-                                                x (Abstract.Closure x0 e0 abs_C') 
+    remember (fun t' => if eqb t' (update C (ST mem t) x (Closure x0 e0 C0))
+                        then Abs.update abs_C abs_st'
+                                        x (Closure x0 e0 abs_C') 
                         else α' t') as α''.
     destruct abs_st as [mem' t']. destruct abs_st' as [mem'' t''].
+    assert (eq_bound_α t α' α'') as EQ''.
+    { red. intros. rewrite Heqα''. 
+      assert (eqb t'0 (update C (ST mem t) x (Closure x0 e0 C0)) = false).
+      refl_bool. unfold "<>". intros contra. rewrite eqb_eq in contra.
+      assert (leb t t'0 = true). rewrite contra. apply update_lt. 
+      assert (t = t'0) as RR. apply leb_sym; eauto. rewrite <- RR in contra.
+      clear RR.
+      assert (eqb t (update C (ST mem t) x (Closure x0 e0 C0)) <> true).
+      refl_bool. apply update_lt. apply H0. rewrite <- contra. apply eqb_refl.
+      rewrite H. eauto. }
     assert (sound α'' (C [|dy_c_lete x t ([||])|])
-            (ST (t :: dy_level C !-> Closure x0 e0 C0; mem) 
-                (update_t C (ST mem t) x (Closure x0 e0 C0)))
-            (abs_C [#| Abstract.dy_c_lete x (α' t) ([#||#]) |#])
-            (Abstract.ST ((α' t) :: Abstract.dy_level abs_C !#-> Abstract.Closure x0 e0 abs_C'; mem'') 
-                         (Abstract.update_t abs_C (Abstract.ST mem'' t'') x (Abstract.Closure x0 e0 abs_C')))).
-    { simpl. unfold update_t in *. repeat split.
-      - rewrite Heqα''. simpl. assert (t =? t = true). rewrite Nat.eqb_eq. eauto. rewrite H. eauto.
+            (ST (t !-> Closure x0 e0 C0; mem) 
+                (update C (ST mem t) x (Closure x0 e0 C0)))
+            (abs_C [| dy_c_lete x (α' t) ([||]) |])
+            (Abs.ST ((α' t) !#-> Closure x0 e0 abs_C'; mem'') 
+                    (Abs.update abs_C (Abs.ST mem'' t'') x (Closure x0 e0 abs_C')))).
+    { simpl. repeat split.
+      - rewrite Heqα''. simpl. rewrite eqb_refl. eauto.
       - rewrite Heqα''. simpl. rewrite plugin_trans_ctx; simpl.
-        assert (t =? S t = false). rewrite Nat.eqb_neq. eauto. rewrite H.
+        assert (eqb t (update C (ST mem t) x (Closure x0 e0 C0)) = false). apply update_lt.
+        rewrite H.
         assert (trans_ctx α'' C = abs_C). 
-        simpl in SOUND. destruct SOUND as [? [RR ?]]. rewrite <- RR.
+        simpl in SOUND. destruct SOUND as [? [RR ?]]. rewrite <- RR. symmetry.
         apply bound_trans_ctx_eq with (t := t0). destruct BOUND. eauto.
-        red. intros. rewrite Heqα''. assert (t'0 <> S t) as RR'. nia. rewrite <- Nat.eqb_neq in RR'. rewrite RR'.
-        symmetry. apply EQ'. eauto. 
-        rewrite Heqα'' in H0. simpl in H0. rewrite H0. eauto.
+        red. intros. rewrite Heqα''. assert (eqb t'0 (update C (ST mem t) x (Closure x0 e0 C0)) = false).
+        refl_bool. unfold "<>". intros contra. rewrite eqb_eq in contra.
+        assert (leb t'0 t = true). lebt t0.
+        assert (t = t'0) as RR'. apply leb_sym; try assumption. rewrite contra. apply update_lt.
+        assert (t < t'0) as contra'. rewrite contra. apply update_lt.
+        destruct contra' as [? contra']. rewrite RR' in contra'. rewrite eqb_refl in contra'. inversion contra'.
+        rewrite H2. apply EQ'. eauto. rewrite <- Heqα''. rewrite H0. eauto.
       - intros. simpl in SOUND. destruct SOUND as [? [? ?]].
                 simpl in SOUND'. destruct SOUND' as [[? [? ?]] ?].
-        unfold update_m. unfold Abstract.update_m.
-        remember (eq_p p (t :: dy_level C)) as b.
-        destruct b. symmetry in Heqb. rewrite eq_p_eq in Heqb.
-        assert (map α'' p =  α' t :: Abstract.dy_level abs_C).
-        rewrite Heqα''. rewrite Heqb. simpl. assert (RR : t =? S t = false). 
-        apply Nat.eqb_neq. eauto. rewrite RR. clear RR. rewrite <- H0.
-        assert (Abstract.dy_level (trans_ctx α C) = map α'' (dy_level C)) as RR.
-        apply level_trans_ctx_eq with (t := t0). red. intros.
-        rewrite Heqα''. assert (t'0 =? S t = false). rewrite Nat.eqb_neq. nia.
-        rewrite H6. apply EQ'. eauto.
-        simpl in BOUND. destruct BOUND. eauto.
-        rewrite RR. rewrite Heqα''. simpl. eauto.
-        (* A bug? in Coq : have to write explicitly the implicit parameters *)
-        assert (Abstract.eq_p (@map time Abstract.time α'' p) (@map nat bool α'' p) = true).
-        rewrite Abstract.eq_p_eq. eauto. rewrite <- H6. rewrite H7. simpl. left.
+        unfold update_m. unfold Abs.update_m.
+        remember (eqb p t) as b.
+        destruct b. symmetry in Heqb. rewrite eqb_eq in Heqb.
+        assert (α' t = α'' p). rewrite Heqb. apply EQ''. apply leb_refl.
+        rewrite H6. rewrite eqb_refl. left.
         assert (abs_C' = trans_ctx α'' C0).
-        rewrite <- H3. eapply bound_trans_ctx_eq. simpl in BOUND'. destruct BOUND'. eauto.
-        rewrite Heqα''. red. intros. assert (t'0 =? S t = false). rewrite Nat.eqb_neq. nia.
-        rewrite H8. eauto. rewrite H8. eauto.
+        rewrite <- H3. eapply bound_trans_ctx_eq. destruct BOUND'. eauto. eauto.
+        rewrite H7. eauto. 
         pose proof (p_bound_or_not p t) as CASES.
         destruct BOUND' as [B1' [B2' B3']].
         destruct CASES as [L | R]; 
@@ -692,45 +722,35 @@ Proof.
         remember (mem p) as access eqn: ACCESS.
         destruct access; eauto; destruct e1; simpl.
         specialize (H4 p L) as HINT. rewrite <- ACCESS in HINT.
-        assert (@map time Abstract.time α'' p = map α' p) as RR.
-        { clear HINT. clear BOUND0. clear Heqb. clear ACCESS.
-          induction p; simpl; eauto. simpl in L; destruct L.
-          rewrite IHp; eauto. rewrite Heqα''. 
-          assert (a =? S t = false). rewrite Nat.eqb_neq. nia.
-          rewrite H8. eauto. } rewrite RR; clear RR.
-        assert (trans_ctx α'' C1 = trans_ctx α' C1) as RR.
-        { apply bound_trans_ctx_eq with (t := t).
-          specialize (B3' p L). rewrite <- ACCESS in B3'. eauto.
-          rewrite Heqα''. red. intros. assert (t'0 =? S t = false).
-          rewrite Nat.eqb_neq. nia. rewrite H6. eauto. } rewrite RR; clear RR.
-        remember (α' t :: Abstract.dy_level abs_C) as p'.
-        remember (Abstract.eq_p (map α' p) p') as b.
+        assert (α'' p = α' p) as RR. 
+        { symmetry. apply EQ''. apply L. } rewrite RR; clear RR.
+        assert (trans_ctx α' C1 = trans_ctx α'' C1) as RR.
+        { apply bound_trans_ctx_eq with (t := t); eauto.
+          specialize (B3' p L). rewrite <- ACCESS in B3'. eauto. } rewrite <- RR; clear RR.
+        remember (α' t) as p'.
+        remember (eqb (α' p) p') as b.
         destruct b. 
-        simpl. right. symmetry in Heqb0. rewrite Abstract.eq_p_eq in Heqb0.
-        rewrite <- Heqb0. apply HINT. apply HINT.
+        simpl. right. symmetry in Heqb0. rewrite eqb_eq in Heqb0.
+        rewrite <- Heqb0. apply HINT; eauto. apply HINT; eauto.
     }
-    assert (eq_bound_α t α' α'') as EQ''.
-    { red. intros. rewrite Heqα''. assert (t'0 =? S t = false). rewrite Nat.eqb_neq. nia.
-      rewrite H0. eauto. }
-    specialize (IHEVAL2 (abs_C [#|Abstract.dy_c_lete x (α' t) ([#||#])|#])
-                (Abstract.ST
-                  (α' t :: Abstract.dy_level abs_C
-                      !#-> Abstract.Closure x0 e0 abs_C'; mem'')
-                  (Abstract.update_t abs_C (Abstract.ST mem'' t'') x
-                  (Abstract.Closure x0 e0 abs_C'))) α'' H).
+    specialize (IHEVAL2 (abs_C [|dy_c_lete x (α' t) ([||])|])
+                (Abs.ST
+                  (α' t !#-> Closure x0 e0 abs_C'; mem'')
+                  (Abs.update abs_C (Abs.ST mem'' t'') x
+                  (Closure x0 e0 abs_C'))) α'' H). clear H.
     destruct IHEVAL2 as [abs_C'' [abs_st'' [α''' [EQ''' SOUND''']]]].
     destruct SOUND' as [SOUND' EVAL'].
     destruct SOUND''' as [SOUND''' EVAL'''].
     exists abs_C''. exists abs_st''. exists α'''. repeat split; eauto.
     red. intros. 
     assert (α t'0 = α' t'0) as RR. apply EQ'. eauto. rewrite RR; clear RR.
-    assert (α' t'0 = α'' t'0) as RR. apply EQ''. nia. rewrite RR; clear RR.
-    apply EQ'''. unfold update_t. nia.
+    assert (α' t'0 = α'' t'0) as RR. apply EQ''. lebt t0. rewrite RR; clear RR.
+    apply EQ'''. lebt t. lebt t0.
     eapply Abstract.Eval_lete; eauto.
     destruct SOUND' as [? [RR ?]]. rewrite RR. 
     destruct abs_st''. destruct SOUND''' as [? [RR' ?]]. rewrite RR' in *.
-    rewrite <- H2. rewrite <- H2 in EVAL'''.
-    rewrite <- H0 in *. exact EVAL'''.
+    rewrite <- H. rewrite <- H in EVAL'''.
+    rewrite <- RR in *. exact EVAL'''.
   - pose proof (time_bound_e C st m' (MVal C') st' EVAL1) as BOUND'.
     pose proof (time_bound_e (C [|dy_c_letm M C' ([||])|]) st' m''
                              (MVal C'') st'' EVAL2) as BOUND''.
@@ -742,7 +762,6 @@ Proof.
             (ST mem0 t0)) as B1.
     { simpl. simpl in BOUND. destruct BOUND as [BB1 [BB2 BB3]].
              simpl in BOUND'. destruct BOUND' as [BB1' [BB2' BB3']].
-      unfold update_t in *.
       split. rewrite plugin_ctx_bound. split.
       eapply relax_ctx_bound. eauto. eauto. simpl. split; eauto. split; eauto. }
     specialize (BOUND'' B1).
@@ -750,7 +769,7 @@ Proof.
     specialize (IHEVAL1 abs_C abs_st α SOUND).
     destruct IHEVAL1 as [abs_C' [abs_st' [α' [EQ' SOUND']]]].
     assert (sound α' (C [|dy_c_letm M C' ([||])|]) (ST mem0 t0)
-            (abs_C [#| Abstract.dy_c_letm M abs_C' ([#||#]) |#]) abs_st').
+            (abs_C [|dy_c_letm M abs_C' ([||]) |]) abs_st').
     { unfold sound in *. destruct abs_st'. destruct abs_st.
       destruct SOUND' as [[? [? ?]] ?].
       destruct SOUND as [? [? ?]].
@@ -766,7 +785,7 @@ Proof.
     }
     assert (eq_bound_α t α' α') as EQ''.
     { red. intros; eauto. }
-    specialize (IHEVAL2 (abs_C [#|Abstract.dy_c_letm M abs_C' ([#||#])|#])
+    specialize (IHEVAL2 (abs_C [|dy_c_letm M abs_C' ([||])|])
                         abs_st' α' H).
     destruct IHEVAL2 as [abs_C'' [abs_st'' [α'' [EQ''' SOUND''']]]].
     destruct SOUND' as [SOUND' EVAL'].
@@ -774,7 +793,7 @@ Proof.
     exists abs_C''. exists abs_st''. exists α''. repeat split; eauto.
     red. intros. 
     assert (α t' = α' t') as RR. apply EQ'. eauto. rewrite RR; clear RR.
-    apply EQ'''. unfold update_t. nia.
+    apply EQ'''. lebt t.
     eapply Abstract.Eval_letm; eauto.
     destruct abs_st'. destruct SOUND' as [? [RR ?]].
     destruct abs_st''. destruct SOUND''' as [? [RR' ?]].
