doc/coq/Syntax.v
@@ -316,6 +316,7 @@ Class OrderT T : Type :=
   leb : T -> T -> bool;
   leb_refl : forall t, leb t t = true;
   leb_trans : forall t t' t'' (LE : leb t t' = true) (LE' : leb t' t'' = true), leb t t'' = true;
+  leb_sym : forall t t' (LE : leb t t' = true) (LE' : leb t' t = true), t = t';
   eqb : T -> T -> bool;
   eqb_eq : forall (t t' : T), eqb t t' = true <-> t = t';
   eqb_neq : forall (t t' : T), eqb t t' = false <-> t <> t'
